iris/WpKvInstr.v
@@ -20,6 +20,7 @@ Require Import WpAdd WpFetch WpLoad WpDecode WpLeafCommon WpEntry.
 Require Import WpGpr WpGprRvc.
 Require Import SmodeCore WpSmodeGpr WpSmodeSret WpEntryNew.
 From Kernel Require KernelInstrs.
+From Kernel Require KernelSyms.
 Local Open Scope Z_scope.
 Import Defs.
 
@@ -414,262 +415,262 @@ Section WpKvInstr.
     | iIntros (? ? ? ?) "_"; iPureIntro; intros; apply decname; assumption ].
 
   Lemma kv_i2 :
-    kernel_text -∗ instr (mword_of_int 0x800053e2 : mword 64) true (C_SDSP (mword_of_int 0 : mword 6, Regidx (mword_of_int 1 : mword 5))).
+    kernel_text -∗ instr (mword_of_int (KernelSyms.kernelvec + 0x2) : mword 64) true (C_SDSP (mword_of_int 0 : mword 6, Regidx (mword_of_int 1 : mword 5))).
   Proof.
-    kv_mk_rvc2 0x800053e2 (mword_of_int 0xe006 : mword 16)
-      (mword_of_int 0x800053e2 : mword 64) (C_SDSP (mword_of_int 0 : mword 6, Regidx (mword_of_int 1 : mword 5))) kv_dec2.
+    kv_mk_rvc2 (KernelSyms.kernelvec + 0x2) (mword_of_int 0xe006 : mword 16)
+      (mword_of_int (KernelSyms.kernelvec + 0x2) : mword 64) (C_SDSP (mword_of_int 0 : mword 6, Regidx (mword_of_int 1 : mword 5))) kv_dec2.
   Qed.
 
   Lemma kv_i3 :
-    kernel_text -∗ instr (mword_of_int 0x800053e4 : mword 64) true (C_SDSP (mword_of_int 2 : mword 6, Regidx (mword_of_int 3 : mword 5))).
+    kernel_text -∗ instr (mword_of_int (KernelSyms.kernelvec + 0x4) : mword 64) true (C_SDSP (mword_of_int 2 : mword 6, Regidx (mword_of_int 3 : mword 5))).
   Proof.
-    kv_mk_rvc4 0x800053e4 (mword_of_int 0xe80e : mword 16) (mword_of_int 0xf016e80e : mword 32)
-      (mword_of_int 0x800053e4 : mword 64) (C_SDSP (mword_of_int 2 : mword 6, Regidx (mword_of_int 3 : mword 5))) kv_dec3.
+    kv_mk_rvc4 (KernelSyms.kernelvec + 0x4) (mword_of_int 0xe80e : mword 16) (mword_of_int 0xf016e80e : mword 32)
+      (mword_of_int (KernelSyms.kernelvec + 0x4) : mword 64) (C_SDSP (mword_of_int 2 : mword 6, Regidx (mword_of_int 3 : mword 5))) kv_dec3.
   Qed.
 
   Lemma kv_i4 :
-    kernel_text -∗ instr (mword_of_int 0x800053e6 : mword 64) true (C_SDSP (mword_of_int 4 : mword 6, Regidx (mword_of_int 5 : mword 5))).
+    kernel_text -∗ instr (mword_of_int (KernelSyms.kernelvec + 0x6) : mword 64) true (C_SDSP (mword_of_int 4 : mword 6, Regidx (mword_of_int 5 : mword 5))).
   Proof.
-    kv_mk_rvc2 0x800053e6 (mword_of_int 0xf016 : mword 16)
-      (mword_of_int 0x800053e6 : mword 64) (C_SDSP (mword_of_int 4 : mword 6, Regidx (mword_of_int 5 : mword 5))) kv_dec4.
+    kv_mk_rvc2 (KernelSyms.kernelvec + 0x6) (mword_of_int 0xf016 : mword 16)
+      (mword_of_int (KernelSyms.kernelvec + 0x6) : mword 64) (C_SDSP (mword_of_int 4 : mword 6, Regidx (mword_of_int 5 : mword 5))) kv_dec4.
   Qed.
 
   Lemma kv_i5 :
-    kernel_text -∗ instr (mword_of_int 0x800053e8 : mword 64) true (C_SDSP (mword_of_int 5 : mword 6, Regidx (mword_of_int 6 : mword 5))).
+    kernel_text -∗ instr (mword_of_int (KernelSyms.kernelvec + 0x8) : mword 64) true (C_SDSP (mword_of_int 5 : mword 6, Regidx (mword_of_int 6 : mword 5))).
   Proof.
-    kv_mk_rvc4 0x800053e8 (mword_of_int 0xf41a : mword 16) (mword_of_int 0xf81ef41a : mword 32)
-      (mword_of_int 0x800053e8 : mword 64) (C_SDSP (mword_of_int 5 : mword 6, Regidx (mword_of_int 6 : mword 5))) kv_dec5.
+    kv_mk_rvc4 (KernelSyms.kernelvec + 0x8) (mword_of_int 0xf41a : mword 16) (mword_of_int 0xf81ef41a : mword 32)
+      (mword_of_int (KernelSyms.kernelvec + 0x8) : mword 64) (C_SDSP (mword_of_int 5 : mword 6, Regidx (mword_of_int 6 : mword 5))) kv_dec5.
   Qed.
 
   Lemma kv_i6 :
-    kernel_text -∗ instr (mword_of_int 0x800053ea : mword 64) true (C_SDSP (mword_of_int 6 : mword 6, Regidx (mword_of_int 7 : mword 5))).
+    kernel_text -∗ instr (mword_of_int (KernelSyms.kernelvec + 0xa) : mword 64) true (C_SDSP (mword_of_int 6 : mword 6, Regidx (mword_of_int 7 : mword 5))).
   Proof.
-    kv_mk_rvc2 0x800053ea (mword_of_int 0xf81e : mword 16)
-      (mword_of_int 0x800053ea : mword 64) (C_SDSP (mword_of_int 6 : mword 6, Regidx (mword_of_int 7 : mword 5))) kv_dec6.
+    kv_mk_rvc2 (KernelSyms.kernelvec + 0xa) (mword_of_int 0xf81e : mword 16)
+      (mword_of_int (KernelSyms.kernelvec + 0xa) : mword 64) (C_SDSP (mword_of_int 6 : mword 6, Regidx (mword_of_int 7 : mword 5))) kv_dec6.
   Qed.
 
   Lemma kv_i7 :
-    kernel_text -∗ instr (mword_of_int 0x800053ec : mword 64) true (C_SDSP (mword_of_int 9 : mword 6, Regidx (mword_of_int 10 : mword 5))).
+    kernel_text -∗ instr (mword_of_int (KernelSyms.kernelvec + 0xc) : mword 64) true (C_SDSP (mword_of_int 9 : mword 6, Regidx (mword_of_int 10 : mword 5))).
   Proof.
-    kv_mk_rvc4 0x800053ec (mword_of_int 0xe4aa : mword 16) (mword_of_int 0xe8aee4aa : mword 32)
-      (mword_of_int 0x800053ec : mword 64) (C_SDSP (mword_of_int 9 : mword 6, Regidx (mword_of_int 10 : mword 5))) kv_dec7.
+    kv_mk_rvc4 (KernelSyms.kernelvec + 0xc) (mword_of_int 0xe4aa : mword 16) (mword_of_int 0xe8aee4aa : mword 32)
+      (mword_of_int (KernelSyms.kernelvec + 0xc) : mword 64) (C_SDSP (mword_of_int 9 : mword 6, Regidx (mword_of_int 10 : mword 5))) kv_dec7.
   Qed.
 
   Lemma kv_i8 :
-    kernel_text -∗ instr (mword_of_int 0x800053ee : mword 64) true (C_SDSP (mword_of_int 10 : mword 6, Regidx (mword_of_int 11 : mword 5))).
+    kernel_text -∗ instr (mword_of_int (KernelSyms.kernelvec + 0xe) : mword 64) true (C_SDSP (mword_of_int 10 : mword 6, Regidx (mword_of_int 11 : mword 5))).
   Proof.
-    kv_mk_rvc2 0x800053ee (mword_of_int 0xe8ae : mword 16)
-      (mword_of_int 0x800053ee : mword 64) (C_SDSP (mword_of_int 10 : mword 6, Regidx (mword_of_int 11 : mword 5))) kv_dec8.
+    kv_mk_rvc2 (KernelSyms.kernelvec + 0xe) (mword_of_int 0xe8ae : mword 16)
+      (mword_of_int (KernelSyms.kernelvec + 0xe) : mword 64) (C_SDSP (mword_of_int 10 : mword 6, Regidx (mword_of_int 11 : mword 5))) kv_dec8.
   Qed.
 
   Lemma kv_i9 :
-    kernel_text -∗ instr (mword_of_int 0x800053f0 : mword 64) true (C_SDSP (mword_of_int 11 : mword 6, Regidx (mword_of_int 12 : mword 5))).
+    kernel_text -∗ instr (mword_of_int (KernelSyms.kernelvec + 0x10) : mword 64) true (C_SDSP (mword_of_int 11 : mword 6, Regidx (mword_of_int 12 : mword 5))).
   Proof.
-    kv_mk_rvc4 0x800053f0 (mword_of_int 0xecb2 : mword 16) (mword_of_int 0xf0b6ecb2 : mword 32)
-      (mword_of_int 0x800053f0 : mword 64) (C_SDSP (mword_of_int 11 : mword 6, Regidx (mword_of_int 12 : mword 5))) kv_dec9.
+    kv_mk_rvc4 (KernelSyms.kernelvec + 0x10) (mword_of_int 0xecb2 : mword 16) (mword_of_int 0xf0b6ecb2 : mword 32)
+      (mword_of_int (KernelSyms.kernelvec + 0x10) : mword 64) (C_SDSP (mword_of_int 11 : mword 6, Regidx (mword_of_int 12 : mword 5))) kv_dec9.
   Qed.
 
   Lemma kv_i10 :
-    kernel_text -∗ instr (mword_of_int 0x800053f2 : mword 64) true (C_SDSP (mword_of_int 12 : mword 6, Regidx (mword_of_int 13 : mword 5))).
+    kernel_text -∗ instr (mword_of_int (KernelSyms.kernelvec + 0x12) : mword 64) true (C_SDSP (mword_of_int 12 : mword 6, Regidx (mword_of_int 13 : mword 5))).
   Proof.
-    kv_mk_rvc2 0x800053f2 (mword_of_int 0xf0b6 : mword 16)
-      (mword_of_int 0x800053f2 : mword 64) (C_SDSP (mword_of_int 12 : mword 6, Regidx (mword_of_int 13 : mword 5))) kv_dec10.
+    kv_mk_rvc2 (KernelSyms.kernelvec + 0x12) (mword_of_int 0xf0b6 : mword 16)
+      (mword_of_int (KernelSyms.kernelvec + 0x12) : mword 64) (C_SDSP (mword_of_int 12 : mword 6, Regidx (mword_of_int 13 : mword 5))) kv_dec10.
   Qed.
 
   Lemma kv_i11 :
-    kernel_text -∗ instr (mword_of_int 0x800053f4 : mword 64) true (C_SDSP (mword_of_int 13 : mword 6, Regidx (mword_of_int 14 : mword 5))).
+    kernel_text -∗ instr (mword_of_int (KernelSyms.kernelvec + 0x14) : mword 64) true (C_SDSP (mword_of_int 13 : mword 6, Regidx (mword_of_int 14 : mword 5))).
   Proof.
-    kv_mk_rvc4 0x800053f4 (mword_of_int 0xf4ba : mword 16) (mword_of_int 0xf8bef4ba : mword 32)
-      (mword_of_int 0x800053f4 : mword 64) (C_SDSP (mword_of_int 13 : mword 6, Regidx (mword_of_int 14 : mword 5))) kv_dec11.
+    kv_mk_rvc4 (KernelSyms.kernelvec + 0x14) (mword_of_int 0xf4ba : mword 16) (mword_of_int 0xf8bef4ba : mword 32)
+      (mword_of_int (KernelSyms.kernelvec + 0x14) : mword 64) (C_SDSP (mword_of_int 13 : mword 6, Regidx (mword_of_int 14 : mword 5))) kv_dec11.
   Qed.
 
   Lemma kv_i12 :
-    kernel_text -∗ instr (mword_of_int 0x800053f6 : mword 64) true (C_SDSP (mword_of_int 14 : mword 6, Regidx (mword_of_int 15 : mword 5))).
+    kernel_text -∗ instr (mword_of_int (KernelSyms.kernelvec + 0x16) : mword 64) true (C_SDSP (mword_of_int 14 : mword 6, Regidx (mword_of_int 15 : mword 5))).
   Proof.
-    kv_mk_rvc2 0x800053f6 (mword_of_int 0xf8be : mword 16)
-      (mword_of_int 0x800053f6 : mword 64) (C_SDSP (mword_of_int 14 : mword 6, Regidx (mword_of_int 15 : mword 5))) kv_dec12.
+    kv_mk_rvc2 (KernelSyms.kernelvec + 0x16) (mword_of_int 0xf8be : mword 16)
+      (mword_of_int (KernelSyms.kernelvec + 0x16) : mword 64) (C_SDSP (mword_of_int 14 : mword 6, Regidx (mword_of_int 15 : mword 5))) kv_dec12.
   Qed.
 
   Lemma kv_i13 :
-    kernel_text -∗ instr (mword_of_int 0x800053f8 : mword 64) true (C_SDSP (mword_of_int 15 : mword 6, Regidx (mword_of_int 16 : mword 5))).
+    kernel_text -∗ instr (mword_of_int (KernelSyms.kernelvec + 0x18) : mword 64) true (C_SDSP (mword_of_int 15 : mword 6, Regidx (mword_of_int 16 : mword 5))).
   Proof.
-    kv_mk_rvc4 0x800053f8 (mword_of_int 0xfcc2 : mword 16) (mword_of_int 0xe146fcc2 : mword 32)
-      (mword_of_int 0x800053f8 : mword 64) (C_SDSP (mword_of_int 15 : mword 6, Regidx (mword_of_int 16 : mword 5))) kv_dec13.
+    kv_mk_rvc4 (KernelSyms.kernelvec + 0x18) (mword_of_int 0xfcc2 : mword 16) (mword_of_int 0xe146fcc2 : mword 32)
+      (mword_of_int (KernelSyms.kernelvec + 0x18) : mword 64) (C_SDSP (mword_of_int 15 : mword 6, Regidx (mword_of_int 16 : mword 5))) kv_dec13.
   Qed.
 
   Lemma kv_i14 :
-    kernel_text -∗ instr (mword_of_int 0x800053fa : mword 64) true (C_SDSP (mword_of_int 16 : mword 6, Regidx (mword_of_int 17 : mword 5))).
+    kernel_text -∗ instr (mword_of_int (KernelSyms.kernelvec + 0x1a) : mword 64) true (C_SDSP (mword_of_int 16 : mword 6, Regidx (mword_of_int 17 : mword 5))).
   Proof.
-    kv_mk_rvc2 0x800053fa (mword_of_int 0xe146 : mword 16)
-      (mword_of_int 0x800053fa : mword 64) (C_SDSP (mword_of_int 16 : mword 6, Regidx (mword_of_int 17 : mword 5))) kv_dec14.
+    kv_mk_rvc2 (KernelSyms.kernelvec + 0x1a) (mword_of_int 0xe146 : mword 16)
+      (mword_of_int (KernelSyms.kernelvec + 0x1a) : mword 64) (C_SDSP (mword_of_int 16 : mword 6, Regidx (mword_of_int 17 : mword 5))) kv_dec14.
   Qed.
 
   Lemma kv_i15 :
-    kernel_text -∗ instr (mword_of_int 0x800053fc : mword 64) true (C_SDSP (mword_of_int 27 : mword 6, Regidx (mword_of_int 28 : mword 5))).
+    kernel_text -∗ instr (mword_of_int (KernelSyms.kernelvec + 0x1c) : mword 64) true (C_SDSP (mword_of_int 27 : mword 6, Regidx (mword_of_int 28 : mword 5))).
   Proof.
-    kv_mk_rvc4 0x800053fc (mword_of_int 0xedf2 : mword 16) (mword_of_int 0xf1f6edf2 : mword 32)
-      (mword_of_int 0x800053fc : mword 64) (C_SDSP (mword_of_int 27 : mword 6, Regidx (mword_of_int 28 : mword 5))) kv_dec15.
+    kv_mk_rvc4 (KernelSyms.kernelvec + 0x1c) (mword_of_int 0xedf2 : mword 16) (mword_of_int 0xf1f6edf2 : mword 32)
+      (mword_of_int (KernelSyms.kernelvec + 0x1c) : mword 64) (C_SDSP (mword_of_int 27 : mword 6, Regidx (mword_of_int 28 : mword 5))) kv_dec15.
   Qed.
 
   Lemma kv_i16 :
-    kernel_text -∗ instr (mword_of_int 0x800053fe : mword 64) true (C_SDSP (mword_of_int 28 : mword 6, Regidx (mword_of_int 29 : mword 5))).
+    kernel_text -∗ instr (mword_of_int (KernelSyms.kernelvec + 0x1e) : mword 64) true (C_SDSP (mword_of_int 28 : mword 6, Regidx (mword_of_int 29 : mword 5))).
   Proof.
-    kv_mk_rvc2 0x800053fe (mword_of_int 0xf1f6 : mword 16)
-      (mword_of_int 0x800053fe : mword 64) (C_SDSP (mword_of_int 28 : mword 6, Regidx (mword_of_int 29 : mword 5))) kv_dec16.
+    kv_mk_rvc2 (KernelSyms.kernelvec + 0x1e) (mword_of_int 0xf1f6 : mword 16)
+      (mword_of_int (KernelSyms.kernelvec + 0x1e) : mword 64) (C_SDSP (mword_of_int 28 : mword 6, Regidx (mword_of_int 29 : mword 5))) kv_dec16.
   Qed.
 
   Lemma kv_i17 :
-    kernel_text -∗ instr (mword_of_int 0x80005400 : mword 64) true (C_SDSP (mword_of_int 29 : mword 6, Regidx (mword_of_int 30 : mword 5))).
+    kernel_text -∗ instr (mword_of_int (KernelSyms.kernelvec + 0x20) : mword 64) true (C_SDSP (mword_of_int 29 : mword 6, Regidx (mword_of_int 30 : mword 5))).
   Proof.
-    kv_mk_rvc4 0x80005400 (mword_of_int 0xf5fa : mword 16) (mword_of_int 0xf9fef5fa : mword 32)
-      (mword_of_int 0x80005400 : mword 64) (C_SDSP (mword_of_int 29 : mword 6, Regidx (mword_of_int 30 : mword 5))) kv_dec17.
+    kv_mk_rvc4 (KernelSyms.kernelvec + 0x20) (mword_of_int 0xf5fa : mword 16) (mword_of_int 0xf9fef5fa : mword 32)
+      (mword_of_int (KernelSyms.kernelvec + 0x20) : mword 64) (C_SDSP (mword_of_int 29 : mword 6, Regidx (mword_of_int 30 : mword 5))) kv_dec17.
   Qed.
 
   Lemma kv_i18 :
-    kernel_text -∗ instr (mword_of_int 0x80005402 : mword 64) true (C_SDSP (mword_of_int 30 : mword 6, Regidx (mword_of_int 31 : mword 5))).
+    kernel_text -∗ instr (mword_of_int (KernelSyms.kernelvec + 0x22) : mword 64) true (C_SDSP (mword_of_int 30 : mword 6, Regidx (mword_of_int 31 : mword 5))).
   Proof.
-    kv_mk_rvc2 0x80005402 (mword_of_int 0xf9fe : mword 16)
-      (mword_of_int 0x80005402 : mword 64) (C_SDSP (mword_of_int 30 : mword 6, Regidx (mword_of_int 31 : mword 5))) kv_dec18.
+    kv_mk_rvc2 (KernelSyms.kernelvec + 0x22) (mword_of_int 0xf9fe : mword 16)
+      (mword_of_int (KernelSyms.kernelvec + 0x22) : mword 64) (C_SDSP (mword_of_int 30 : mword 6, Regidx (mword_of_int 31 : mword 5))) kv_dec18.
   Qed.
 
   Lemma kv_i19 :
-    kernel_text -∗ instr (mword_of_int 0x80005404 : mword 64) false (JAL (mword_of_int 0x1fd29e : mword 21, Regidx (mword_of_int 1 : mword 5))).
+    kernel_text -∗ instr (mword_of_int (KernelSyms.kernelvec + 0x24) : mword 64) false (JAL (mword_of_int 0x1fd29e : mword 21, Regidx (mword_of_int 1 : mword 5))).
   Proof.
-    kv_mk_base 0x80005404 (mword_of_int 0xa9efd0ef : mword 32)
-      (mword_of_int 0x80005404 : mword 64) (JAL (mword_of_int 0x1fd29e : mword 21, Regidx (mword_of_int 1 : mword 5))) kv_dec19.
+    kv_mk_base (KernelSyms.kernelvec + 0x24) (mword_of_int 0xa9efd0ef : mword 32)
+      (mword_of_int (KernelSyms.kernelvec + 0x24) : mword 64) (JAL (mword_of_int 0x1fd29e : mword 21, Regidx (mword_of_int 1 : mword 5))) kv_dec19.
   Qed.
 
   Lemma kv_i20 :
-    kernel_text -∗ instr (mword_of_int 0x80005408 : mword 64) true (C_LDSP (mword_of_int 0 : mword 6, Regidx (mword_of_int 1 : mword 5))).
+    kernel_text -∗ instr (mword_of_int (KernelSyms.kernelvec + 0x28) : mword 64) true (C_LDSP (mword_of_int 0 : mword 6, Regidx (mword_of_int 1 : mword 5))).
   Proof.
-    kv_mk_rvc4 0x80005408 (mword_of_int 0x6082 : mword 16) (mword_of_int 0x61c26082 : mword 32)
-      (mword_of_int 0x80005408 : mword 64) (C_LDSP (mword_of_int 0 : mword 6, Regidx (mword_of_int 1 : mword 5))) kv_dec20.
+    kv_mk_rvc4 (KernelSyms.kernelvec + 0x28) (mword_of_int 0x6082 : mword 16) (mword_of_int 0x61c26082 : mword 32)
+      (mword_of_int (KernelSyms.kernelvec + 0x28) : mword 64) (C_LDSP (mword_of_int 0 : mword 6, Regidx (mword_of_int 1 : mword 5))) kv_dec20.
   Qed.
 
   Lemma kv_i21 :
-    kernel_text -∗ instr (mword_of_int 0x8000540a : mword 64) true (C_LDSP (mword_of_int 2 : mword 6, Regidx (mword_of_int 3 : mword 5))).
+    kernel_text -∗ instr (mword_of_int (KernelSyms.kernelvec + 0x2a) : mword 64) true (C_LDSP (mword_of_int 2 : mword 6, Regidx (mword_of_int 3 : mword 5))).
   Proof.
-    kv_mk_rvc2 0x8000540a (mword_of_int 0x61c2 : mword 16)
-      (mword_of_int 0x8000540a : mword 64) (C_LDSP (mword_of_int 2 : mword 6, Regidx (mword_of_int 3 : mword 5))) kv_dec21.
+    kv_mk_rvc2 (KernelSyms.kernelvec + 0x2a) (mword_of_int 0x61c2 : mword 16)
+      (mword_of_int (KernelSyms.kernelvec + 0x2a) : mword 64) (C_LDSP (mword_of_int 2 : mword 6, Regidx (mword_of_int 3 : mword 5))) kv_dec21.
   Qed.
 
   Lemma kv_i22 :
-    kernel_text -∗ instr (mword_of_int 0x8000540c : mword 64) true (C_LDSP (mword_of_int 4 : mword 6, Regidx (mword_of_int 5 : mword 5))).
+    kernel_text -∗ instr (mword_of_int (KernelSyms.kernelvec + 0x2c) : mword 64) true (C_LDSP (mword_of_int 4 : mword 6, Regidx (mword_of_int 5 : mword 5))).
   Proof.
-    kv_mk_rvc4 0x8000540c (mword_of_int 0x7282 : mword 16) (mword_of_int 0x73227282 : mword 32)
-      (mword_of_int 0x8000540c : mword 64) (C_LDSP (mword_of_int 4 : mword 6, Regidx (mword_of_int 5 : mword 5))) kv_dec22.
+    kv_mk_rvc4 (KernelSyms.kernelvec + 0x2c) (mword_of_int 0x7282 : mword 16) (mword_of_int 0x73227282 : mword 32)
+      (mword_of_int (KernelSyms.kernelvec + 0x2c) : mword 64) (C_LDSP (mword_of_int 4 : mword 6, Regidx (mword_of_int 5 : mword 5))) kv_dec22.
   Qed.
 
   Lemma kv_i23 :
-    kernel_text -∗ instr (mword_of_int 0x8000540e : mword 64) true (C_LDSP (mword_of_int 5 : mword 6, Regidx (mword_of_int 6 : mword 5))).
+    kernel_text -∗ instr (mword_of_int (KernelSyms.kernelvec + 0x2e) : mword 64) true (C_LDSP (mword_of_int 5 : mword 6, Regidx (mword_of_int 6 : mword 5))).
   Proof.
-    kv_mk_rvc2 0x8000540e (mword_of_int 0x7322 : mword 16)
-      (mword_of_int 0x8000540e : mword 64) (C_LDSP (mword_of_int 5 : mword 6, Regidx (mword_of_int 6 : mword 5))) kv_dec23.
+    kv_mk_rvc2 (KernelSyms.kernelvec + 0x2e) (mword_of_int 0x7322 : mword 16)
+      (mword_of_int (KernelSyms.kernelvec + 0x2e) : mword 64) (C_LDSP (mword_of_int 5 : mword 6, Regidx (mword_of_int 6 : mword 5))) kv_dec23.
   Qed.
 
   Lemma kv_i24 :
-    kernel_text -∗ instr (mword_of_int 0x80005410 : mword 64) true (C_LDSP (mword_of_int 6 : mword 6, Regidx (mword_of_int 7 : mword 5))).
+    kernel_text -∗ instr (mword_of_int (KernelSyms.kernelvec + 0x30) : mword 64) true (C_LDSP (mword_of_int 6 : mword 6, Regidx (mword_of_int 7 : mword 5))).
   Proof.
-    kv_mk_rvc4 0x80005410 (mword_of_int 0x73c2 : mword 16) (mword_of_int 0x652673c2 : mword 32)
-      (mword_of_int 0x80005410 : mword 64) (C_LDSP (mword_of_int 6 : mword 6, Regidx (mword_of_int 7 : mword 5))) kv_dec24.
+    kv_mk_rvc4 (KernelSyms.kernelvec + 0x30) (mword_of_int 0x73c2 : mword 16) (mword_of_int 0x652673c2 : mword 32)
+      (mword_of_int (KernelSyms.kernelvec + 0x30) : mword 64) (C_LDSP (mword_of_int 6 : mword 6, Regidx (mword_of_int 7 : mword 5))) kv_dec24.
   Qed.
 
   Lemma kv_i25 :
-    kernel_text -∗ instr (mword_of_int 0x80005412 : mword 64) true (C_LDSP (mword_of_int 9 : mword 6, Regidx (mword_of_int 10 : mword 5))).
+    kernel_text -∗ instr (mword_of_int (KernelSyms.kernelvec + 0x32) : mword 64) true (C_LDSP (mword_of_int 9 : mword 6, Regidx (mword_of_int 10 : mword 5))).
   Proof.
-    kv_mk_rvc2 0x80005412 (mword_of_int 0x6526 : mword 16)
-      (mword_of_int 0x80005412 : mword 64) (C_LDSP (mword_of_int 9 : mword 6, Regidx (mword_of_int 10 : mword 5))) kv_dec25.
+    kv_mk_rvc2 (KernelSyms.kernelvec + 0x32) (mword_of_int 0x6526 : mword 16)
+      (mword_of_int (KernelSyms.kernelvec + 0x32) : mword 64) (C_LDSP (mword_of_int 9 : mword 6, Regidx (mword_of_int 10 : mword 5))) kv_dec25.
   Qed.
 
   Lemma kv_i26 :
-    kernel_text -∗ instr (mword_of_int 0x80005414 : mword 64) true (C_LDSP (mword_of_int 10 : mword 6, Regidx (mword_of_int 11 : mword 5))).
+    kernel_text -∗ instr (mword_of_int (KernelSyms.kernelvec + 0x34) : mword 64) true (C_LDSP (mword_of_int 10 : mword 6, Regidx (mword_of_int 11 : mword 5))).
   Proof.
-    kv_mk_rvc4 0x80005414 (mword_of_int 0x65c6 : mword 16) (mword_of_int 0x666665c6 : mword 32)
-      (mword_of_int 0x80005414 : mword 64) (C_LDSP (mword_of_int 10 : mword 6, Regidx (mword_of_int 11 : mword 5))) kv_dec26.
+    kv_mk_rvc4 (KernelSyms.kernelvec + 0x34) (mword_of_int 0x65c6 : mword 16) (mword_of_int 0x666665c6 : mword 32)
+      (mword_of_int (KernelSyms.kernelvec + 0x34) : mword 64) (C_LDSP (mword_of_int 10 : mword 6, Regidx (mword_of_int 11 : mword 5))) kv_dec26.
   Qed.
 
   Lemma kv_i27 :
-    kernel_text -∗ instr (mword_of_int 0x80005416 : mword 64) true (C_LDSP (mword_of_int 11 : mword 6, Regidx (mword_of_int 12 : mword 5))).
+    kernel_text -∗ instr (mword_of_int (KernelSyms.kernelvec + 0x36) : mword 64) true (C_LDSP (mword_of_int 11 : mword 6, Regidx (mword_of_int 12 : mword 5))).
   Proof.
-    kv_mk_rvc2 0x80005416 (mword_of_int 0x6666 : mword 16)
-      (mword_of_int 0x80005416 : mword 64) (C_LDSP (mword_of_int 11 : mword 6, Regidx (mword_of_int 12 : mword 5))) kv_dec27.
+    kv_mk_rvc2 (KernelSyms.kernelvec + 0x36) (mword_of_int 0x6666 : mword 16)
+      (mword_of_int (KernelSyms.kernelvec + 0x36) : mword 64) (C_LDSP (mword_of_int 11 : mword 6, Regidx (mword_of_int 12 : mword 5))) kv_dec27.
   Qed.
 
   Lemma kv_i28 :
-    kernel_text -∗ instr (mword_of_int 0x80005418 : mword 64) true (C_LDSP (mword_of_int 12 : mword 6, Regidx (mword_of_int 13 : mword 5))).
+    kernel_text -∗ instr (mword_of_int (KernelSyms.kernelvec + 0x38) : mword 64) true (C_LDSP (mword_of_int 12 : mword 6, Regidx (mword_of_int 13 : mword 5))).
   Proof.
-    kv_mk_rvc4 0x80005418 (mword_of_int 0x7686 : mword 16) (mword_of_int 0x77267686 : mword 32)
-      (mword_of_int 0x80005418 : mword 64) (C_LDSP (mword_of_int 12 : mword 6, Regidx (mword_of_int 13 : mword 5))) kv_dec28.
+    kv_mk_rvc4 (KernelSyms.kernelvec + 0x38) (mword_of_int 0x7686 : mword 16) (mword_of_int 0x77267686 : mword 32)
+      (mword_of_int (KernelSyms.kernelvec + 0x38) : mword 64) (C_LDSP (mword_of_int 12 : mword 6, Regidx (mword_of_int 13 : mword 5))) kv_dec28.
   Qed.
 
   Lemma kv_i29 :
-    kernel_text -∗ instr (mword_of_int 0x8000541a : mword 64) true (C_LDSP (mword_of_int 13 : mword 6, Regidx (mword_of_int 14 : mword 5))).
+    kernel_text -∗ instr (mword_of_int (KernelSyms.kernelvec + 0x3a) : mword 64) true (C_LDSP (mword_of_int 13 : mword 6, Regidx (mword_of_int 14 : mword 5))).
   Proof.
-    kv_mk_rvc2 0x8000541a (mword_of_int 0x7726 : mword 16)
-      (mword_of_int 0x8000541a : mword 64) (C_LDSP (mword_of_int 13 : mword 6, Regidx (mword_of_int 14 : mword 5))) kv_dec29.
+    kv_mk_rvc2 (KernelSyms.kernelvec + 0x3a) (mword_of_int 0x7726 : mword 16)
+      (mword_of_int (KernelSyms.kernelvec + 0x3a) : mword 64) (C_LDSP (mword_of_int 13 : mword 6, Regidx (mword_of_int 14 : mword 5))) kv_dec29.
   Qed.
 
   Lemma kv_i30 :
-    kernel_text -∗ instr (mword_of_int 0x8000541c : mword 64) true (C_LDSP (mword_of_int 14 : mword 6, Regidx (mword_of_int 15 : mword 5))).
+    kernel_text -∗ instr (mword_of_int (KernelSyms.kernelvec + 0x3c) : mword 64) true (C_LDSP (mword_of_int 14 : mword 6, Regidx (mword_of_int 15 : mword 5))).
   Proof.
-    kv_mk_rvc4 0x8000541c (mword_of_int 0x77c6 : mword 16) (mword_of_int 0x786677c6 : mword 32)
-      (mword_of_int 0x8000541c : mword 64) (C_LDSP (mword_of_int 14 : mword 6, Regidx (mword_of_int 15 : mword 5))) kv_dec30.
+    kv_mk_rvc4 (KernelSyms.kernelvec + 0x3c) (mword_of_int 0x77c6 : mword 16) (mword_of_int 0x786677c6 : mword 32)
+      (mword_of_int (KernelSyms.kernelvec + 0x3c) : mword 64) (C_LDSP (mword_of_int 14 : mword 6, Regidx (mword_of_int 15 : mword 5))) kv_dec30.
   Qed.
 
   Lemma kv_i31 :
-    kernel_text -∗ instr (mword_of_int 0x8000541e : mword 64) true (C_LDSP (mword_of_int 15 : mword 6, Regidx (mword_of_int 16 : mword 5))).
+    kernel_text -∗ instr (mword_of_int (KernelSyms.kernelvec + 0x3e) : mword 64) true (C_LDSP (mword_of_int 15 : mword 6, Regidx (mword_of_int 16 : mword 5))).
   Proof.
-    kv_mk_rvc2 0x8000541e (mword_of_int 0x7866 : mword 16)
-      (mword_of_int 0x8000541e : mword 64) (C_LDSP (mword_of_int 15 : mword 6, Regidx (mword_of_int 16 : mword 5))) kv_dec31.
+    kv_mk_rvc2 (KernelSyms.kernelvec + 0x3e) (mword_of_int 0x7866 : mword 16)
+      (mword_of_int (KernelSyms.kernelvec + 0x3e) : mword 64) (C_LDSP (mword_of_int 15 : mword 6, Regidx (mword_of_int 16 : mword 5))) kv_dec31.
   Qed.
 
   Lemma kv_i32 :
-    kernel_text -∗ instr (mword_of_int 0x80005420 : mword 64) true (C_LDSP (mword_of_int 16 : mword 6, Regidx (mword_of_int 17 : mword 5))).
+    kernel_text -∗ instr (mword_of_int (KernelSyms.kernelvec + 0x40) : mword 64) true (C_LDSP (mword_of_int 16 : mword 6, Regidx (mword_of_int 17 : mword 5))).
   Proof.
-    kv_mk_rvc4 0x80005420 (mword_of_int 0x688a : mword 16) (mword_of_int 0x6e6e688a : mword 32)
-      (mword_of_int 0x80005420 : mword 64) (C_LDSP (mword_of_int 16 : mword 6, Regidx (mword_of_int 17 : mword 5))) kv_dec32.
+    kv_mk_rvc4 (KernelSyms.kernelvec + 0x40) (mword_of_int 0x688a : mword 16) (mword_of_int 0x6e6e688a : mword 32)
+      (mword_of_int (KernelSyms.kernelvec + 0x40) : mword 64) (C_LDSP (mword_of_int 16 : mword 6, Regidx (mword_of_int 17 : mword 5))) kv_dec32.
   Qed.
 
   Lemma kv_i33 :
-    kernel_text -∗ instr (mword_of_int 0x80005422 : mword 64) true (C_LDSP (mword_of_int 27 : mword 6, Regidx (mword_of_int 28 : mword 5))).
+    kernel_text -∗ instr (mword_of_int (KernelSyms.kernelvec + 0x42) : mword 64) true (C_LDSP (mword_of_int 27 : mword 6, Regidx (mword_of_int 28 : mword 5))).
   Proof.
-    kv_mk_rvc2 0x80005422 (mword_of_int 0x6e6e : mword 16)
-      (mword_of_int 0x80005422 : mword 64) (C_LDSP (mword_of_int 27 : mword 6, Regidx (mword_of_int 28 : mword 5))) kv_dec33.
+    kv_mk_rvc2 (KernelSyms.kernelvec + 0x42) (mword_of_int 0x6e6e : mword 16)
+      (mword_of_int (KernelSyms.kernelvec + 0x42) : mword 64) (C_LDSP (mword_of_int 27 : mword 6, Regidx (mword_of_int 28 : mword 5))) kv_dec33.
   Qed.
 
   Lemma kv_i34 :
-    kernel_text -∗ instr (mword_of_int 0x80005424 : mword 64) true (C_LDSP (mword_of_int 28 : mword 6, Regidx (mword_of_int 29 : mword 5))).
+    kernel_text -∗ instr (mword_of_int (KernelSyms.kernelvec + 0x44) : mword 64) true (C_LDSP (mword_of_int 28 : mword 6, Regidx (mword_of_int 29 : mword 5))).
   Proof.
-    kv_mk_rvc4 0x80005424 (mword_of_int 0x7e8e : mword 16) (mword_of_int 0x7f2e7e8e : mword 32)
-      (mword_of_int 0x80005424 : mword 64) (C_LDSP (mword_of_int 28 : mword 6, Regidx (mword_of_int 29 : mword 5))) kv_dec34.
+    kv_mk_rvc4 (KernelSyms.kernelvec + 0x44) (mword_of_int 0x7e8e : mword 16) (mword_of_int 0x7f2e7e8e : mword 32)
+      (mword_of_int (KernelSyms.kernelvec + 0x44) : mword 64) (C_LDSP (mword_of_int 28 : mword 6, Regidx (mword_of_int 29 : mword 5))) kv_dec34.
   Qed.
 
   Lemma kv_i35 :
-    kernel_text -∗ instr (mword_of_int 0x80005426 : mword 64) true (C_LDSP (mword_of_int 29 : mword 6, Regidx (mword_of_int 30 : mword 5))).
+    kernel_text -∗ instr (mword_of_int (KernelSyms.kernelvec + 0x46) : mword 64) true (C_LDSP (mword_of_int 29 : mword 6, Regidx (mword_of_int 30 : mword 5))).
   Proof.
-    kv_mk_rvc2 0x80005426 (mword_of_int 0x7f2e : mword 16)
-      (mword_of_int 0x80005426 : mword 64) (C_LDSP (mword_of_int 29 : mword 6, Regidx (mword_of_int 30 : mword 5))) kv_dec35.
+    kv_mk_rvc2 (KernelSyms.kernelvec + 0x46) (mword_of_int 0x7f2e : mword 16)
+      (mword_of_int (KernelSyms.kernelvec + 0x46) : mword 64) (C_LDSP (mword_of_int 29 : mword 6, Regidx (mword_of_int 30 : mword 5))) kv_dec35.
   Qed.
 
   Lemma kv_i36 :
-    kernel_text -∗ instr (mword_of_int 0x80005428 : mword 64) true (C_LDSP (mword_of_int 30 : mword 6, Regidx (mword_of_int 31 : mword 5))).
+    kernel_text -∗ instr (mword_of_int (KernelSyms.kernelvec + 0x48) : mword 64) true (C_LDSP (mword_of_int 30 : mword 6, Regidx (mword_of_int 31 : mword 5))).
   Proof.
-    kv_mk_rvc4 0x80005428 (mword_of_int 0x7fce : mword 16) (mword_of_int 0x61117fce : mword 32)
-      (mword_of_int 0x80005428 : mword 64) (C_LDSP (mword_of_int 30 : mword 6, Regidx (mword_of_int 31 : mword 5))) kv_dec36.
+    kv_mk_rvc4 (KernelSyms.kernelvec + 0x48) (mword_of_int 0x7fce : mword 16) (mword_of_int 0x61117fce : mword 32)
+      (mword_of_int (KernelSyms.kernelvec + 0x48) : mword 64) (C_LDSP (mword_of_int 30 : mword 6, Regidx (mword_of_int 31 : mword 5))) kv_dec36.
   Qed.
 
   Lemma kv_i37 :
-    kernel_text -∗ instr (mword_of_int 0x8000542a : mword 64) true (C_ADDI16SP (mword_of_int 16 : mword 6)).
+    kernel_text -∗ instr (mword_of_int (KernelSyms.kernelvec + 0x4a) : mword 64) true (C_ADDI16SP (mword_of_int 16 : mword 6)).
   Proof.
-    kv_mk_rvc2 0x8000542a (mword_of_int 0x6111 : mword 16)
-      (mword_of_int 0x8000542a : mword 64) (C_ADDI16SP (mword_of_int 16 : mword 6)) kv_dec37.
+    kv_mk_rvc2 (KernelSyms.kernelvec + 0x4a) (mword_of_int 0x6111 : mword 16)
+      (mword_of_int (KernelSyms.kernelvec + 0x4a) : mword 64) (C_ADDI16SP (mword_of_int 16 : mword 6)) kv_dec37.
   Qed.
 
   Lemma kv_i38 :
-    kernel_text -∗ instr (mword_of_int 0x8000542c : mword 64) false (SRET tt).
+    kernel_text -∗ instr (mword_of_int (KernelSyms.kernelvec + 0x4c) : mword 64) false (SRET tt).
   Proof.
-    kv_mk_base 0x8000542c (mword_of_int 0x10200073 : mword 32)
-      (mword_of_int 0x8000542c : mword 64) (SRET tt) kv_dec38.
+    kv_mk_base (KernelSyms.kernelvec + 0x4c) (mword_of_int 0x10200073 : mword 32)
+      (mword_of_int (KernelSyms.kernelvec + 0x4c) : mword 64) (SRET tt) kv_dec38.
   Qed.
 
 End WpKvInstr.
